AwsCryptographicMaterialProviders/dafny/AwsCryptographicMaterialProviders/test/Keyrings/AwsKms/TestAwsKmsUtils.dfy
@@ -1,0 +1,33 @@
+// Copyright Amazon.com Inc. or its affiliates. All Rights Reserved.
+// SPDX-License-Identifier: Apache-2.0
+
+include "../../../src/Keyrings/AwsKms/AwsKmsUtils.dfy"
+include "../../../../AwsCryptographyKeyStore/test/Fixtures.dfy"
+
+// These tests are not really needed,
+// as proofs cover this logic.
+// However, it helps to clarify how to use these.
+module TestAwsKmsUtils {
+  import opened Fixtures
+  import opened Wrappers
+  import opened AwsKmsUtils
+
+  method {:test} ValidateKmsKeyIdKeyArnSuccess() {
+    var actual :- expect ValidateKmsKeyId(postalHornKeyArn);
+  }
+
+  method {:test} ValidateKmsKeyIdAliasSuccess() {
+    var actual :- expect ValidateKmsKeyId(kmsKeyAlias);
+  }
+
+  method {:test} ValidateKmsKeyIdFractionOfKeyFails() {
+    var actual := ValidateKmsKeyId("key/bc127593-f7da-452c-a1f3-cd34c46f81f8");
+    expect actual.Failure?;
+    actual := ValidateKmsKeyId("370957321024:key/bc127593-f7da-452c-a1f3-cd34c46f81f8");
+    expect actual.Failure?;
+    actual := ValidateKmsKeyId("us-west-2:370957321024:key/bc127593-f7da-452c-a1f3-cd34c46f81f8");
+    expect actual.Failure?;
+    actual := ValidateKmsKeyId("kms:us-west-2:370957321024:key/bc127593-f7da-452c-a1f3-cd34c46f81f8");
+    expect actual.Failure?;
+  }
+}
