AwsCryptographicMaterialProviders/dafny/AwsCryptographicMaterialProviders/test/TestAwsArnParsing.dfy
@@ -1,0 +1,50 @@
+// Copyright Amazon.com Inc. or its affiliates. All Rights Reserved.
+// SPDX-License-Identifier: Apache-2.0
+
+include "../src/AwsArnParsing.dfy"
+include "../../AwsCryptographyKeyStore/test/Fixtures.dfy"
+
+// These tests are not really needed,
+// as proofs cover this logic.
+// However, it helps to clarify how to use these.
+module TestAwsArnParsing {
+  import opened AwsArnParsing
+  import opened Fixtures
+  import opened Wrappers
+  
+  method {:test} ParseAwsKmsIdentifierAliasSuccess() {
+    var actual :- expect ParseAwsKmsIdentifier(kmsKeyAlias);
+  }
+
+  method {:test} ParseAwsKmsArnAliasSuccess() {
+    var actual :- expect ParseAwsKmsArn(kmsKeyAlias);
+    expect actual.region == "us-west-2";
+    expect actual.resource.resourceType == "alias";
+    expect actual.resource.value == "postalHorn";
+  }
+
+  method {:test} ParseAwsKmsArnKeySuccess() {
+    var actual :- expect ParseAwsKmsArn(postalHornKeyArn);
+    expect actual.region == "us-west-2";
+    expect actual.resource.resourceType == "key";
+    expect actual.resource.value == "bc127593-f7da-452c-a1f3-cd34c46f81f8";
+  }
+
+  method {:test} ParseAwsKmsArnFractionOfAliasFails() {
+    var actual := ParseAwsKmsArn("alias/postalHorn");
+    expect actual.Failure?;
+    expect actual.error == "Malformed arn: alias/postalHorn";
+  }
+
+  method {:test} ParseAwsKmsArnFractionOfKeyFails() {
+    var actual := ParseAwsKmsArn("key/bc127593-f7da-452c-a1f3-cd34c46f81f8");
+    expect actual.Failure?;
+    expect actual.error == "Malformed arn: key/bc127593-f7da-452c-a1f3-cd34c46f81f8";
+    actual := ParseAwsKmsArn("370957321024:key/bc127593-f7da-452c-a1f3-cd34c46f81f8");
+    expect actual.Failure?;
+    actual := ParseAwsKmsArn("us-west-2:370957321024:key/bc127593-f7da-452c-a1f3-cd34c46f81f8");
+    expect actual.Failure?;
+    actual := ParseAwsKmsArn("kms:us-west-2:370957321024:key/bc127593-f7da-452c-a1f3-cd34c46f81f8");
+    expect actual.Failure?;
+  }
+}
